Update MinimalLogic.v
mechanized deduction for minimal logic

MinimalLogic.v
@@ -1,91 +1,133 @@
-(* Minimal Logic *)
+From Coq Require Import List.
+Import ListNotations.
+
 
 Definition iffT (X Y : Type) : Type := (X -> Y) * (Y -> X).
 Notation "X <=> Y" := (iffT X Y) (at level 95, no associativity).
 
-
+(* Minimal Logic *)
 Section Minimal.
 
-  (* We try to work in a logic without False and use the variable F in its place *)
-  Variable F : Type.
+  Inductive prop : Type :=
+  | P : nat -> prop
+  | Impl : prop -> prop -> prop
+  | Conj : prop -> prop -> prop
+  | Disj : prop -> prop -> prop.
 
-  Definition Contradiction := forall A B, (A -> F) -> A -> B.
-  Definition Explosion := forall A, F -> A. 
-  Definition LEM := forall A, A + (A -> F).
-  Definition DN := forall A, ((A -> F) -> F) -> A.
-  Definition CP := forall A B, ((B -> F) -> (A -> F)) -> A -> B.
+  Notation "A ∧ B" := (Conj A B) (at level 41).
+  Notation "A ∨ B" := (Disj A B) (at level 42).
+  Notation "A '-->' B" := (Impl A B) (at level 43, right associativity).
+  Notation "x 'el' A" := (In x A) (at level 70).
+  Notation "A <<= B" := (incl A B) (at level 70).
 
-  Definition Peirce := forall A B, ((A -> B) -> A) -> A.
+  (* Inductive type formalizing deduction in minimal logic *)
+  Reserved Notation "A ⊢ s" (at level 70).
+  Inductive prv : list prop -> prop -> Type :=
+  | II A phi psi : phi::A ⊢ psi -> A ⊢ phi --> psi
+  | IE A phi psi : A ⊢ phi --> psi -> A ⊢ phi -> A ⊢ psi
+  | Ctx A phi : phi el A -> A ⊢ phi
+  | CI A phi psi : A ⊢ phi -> A ⊢ psi -> A ⊢ phi ∧ psi
+  | CE1 A phi psi : A ⊢ phi ∧ psi -> A ⊢ phi
+  | CE2 A phi psi : A ⊢ phi ∧ psi -> A ⊢ psi
+  | DI1 A phi psi : A ⊢ phi -> A ⊢ phi ∨ psi
+  | DI2 A phi psi : A ⊢ psi -> A ⊢ phi ∨ psi
+  | DE  A phi psi theta : A ⊢ phi ∨ psi -> phi::A ⊢ theta -> psi::A ⊢ theta -> A ⊢ theta
+  where "A ⊢ phi" := (prv A phi).
 
+  
+  Lemma Weak A B phi :
+    A ⊢ phi -> A <<= B -> B ⊢ phi.
+  Proof.
+    intros H. revert B.
+    induction H; intros B HB; try unshelve (solve [econstructor; intuition]); try now econstructor.
+  Qed.
 
-  Goal Contradiction <=> Explosion.
+    
+  Fact Imp A s t :
+    A ⊢ s --> t <=> s::A ⊢ t.
   Proof.
     split.
-    - intros con A. apply con. auto.
-    - intros expl. intros A B H a. apply expl. auto.
+    - intros H. eapply IE. 2: apply Ctx. eapply Weak. exact H.
+      all: firstorder.
+    - apply II.
+  Qed.
+
+  
+  
+  (* Fix some propositional variable F *)
+  Variable F : prop.
+
+  Definition Contradiction := forall A B, nil ⊢ A --> (F --> A) --> B.
+  Definition Explosion := forall A, nil ⊢ F --> A. 
+  Definition LEM := forall A, nil ⊢ A ∨ (A --> F).
+  Definition DN := forall A, nil ⊢ ((A --> F) --> F) --> A.
+  Definition CP := forall A B, nil ⊢ ((B --> F) --> (A --> F)) --> A --> B.
+
+  Definition Peirce := forall A B, nil ⊢ ((A --> B) --> A) --> A.
+
+
+  Lemma CP' {X Y Gamma} : CP -> Gamma ⊢ (Y --> F) --> (X --> F) -> Gamma ⊢ X --> Y.
+  Proof.
+    intros cp. apply IE. eapply Weak.
+    apply (cp X Y). firstorder.
+  Qed.
+  
+  
+  Goal DN <=> CP.
+  Proof.
+    split.
+    - intros dn A B.
+      generalize (dn B). 
+      eapply IE, II, II, II, IE.
+      apply Ctx; firstorder.
+      eapply II, IE. instantiate (1 := A).
+      eapply IE. all: apply Ctx; firstorder.
+    - intros cp A. apply (CP' cp).
+      eapply II, II, (IE _ (_ --> _)).
+      apply Ctx; firstorder.
+      apply Ctx; firstorder.
+  Qed.
+
+  
+  Goal DN -> Explosion.
+  Proof.
+    intros dn A.
+    generalize (dn A).
+    eapply IE, II, II.
+    eapply IE. apply Ctx; firstorder.
+    apply II, Ctx; firstorder.
   Qed.
   
 
-  Goal DN -> Explosion.
+  Goal CP -> Peirce.
   Proof.
-    intros dn A f. apply dn. intros H. exact f.
+    intros cp A B. apply (CP' cp).
+    eapply II, II, IE. apply Ctx; firstorder.
+    eapply IE. apply Ctx; firstorder.
+    apply (CP' cp). apply II, Ctx. firstorder.
   Qed.
-
+    
+  
+  Goal Peirce -> LEM.
+  Proof.
+    intros peirce X.
+    eapply IE. apply (peirce (X ∨ (X --> F)) F).
+    eapply II, DI2, II, IE. apply Ctx; firstorder.
+    apply DI1, Ctx; firstorder.
+  Qed.
+  
 
   Goal LEM * Explosion -> DN.
   Proof.
-    intros [lem exp] X nnX. destruct (lem X) as [x | H]. exact x.
-    apply exp. apply nnX. exact H.
-  Qed.
-
-  
-  Lemma DN_CP : DN <=> CP.
-  Proof.
-    split.
-    - intros dn X Y cp x. apply dn. intro nY. apply cp. exact nY. exact x.
-    - intros cp X. apply cp. intros nX nnX. apply nnX. exact nX. 
-  Qed.
-
-  
-  Lemma CP_Peirce : CP -> Peirce.
-  Proof.
-    intros cp X Y. apply cp. intros notX H. apply notX, H. apply cp.
-    intro. exact notX.
-  Qed.
-
-
-  Lemma Peirce_LEM : Peirce -> LEM.
-  Proof.
-    intros peirce X. apply (peirce _ F). intro H. right. intros x. apply H.
-    left. exact x. 
+    intros [lem expl] X.
+    generalize (lem X); apply IE.
+    generalize (expl X); apply IE.
+    eapply II, II, II, DE. apply Ctx; firstorder.
+    - apply Ctx; firstorder.
+    - eapply IE. apply Ctx; firstorder.
+      eapply IE. apply (Ctx _ ((X --> F) --> _)); firstorder.
+      apply Ctx; firstorder.
   Qed.
 
 
 End Minimal.
-
-
-(* The above statements are equivalent in intuitionistic logic, 
-when we take F = False. We now show the missing equivalences. *)
-
-
-Definition LEM' := LEM False.
-Definition DN' := DN False.
-Definition CP' := CP False.
-
-
-Goal Peirce <=> CP'.
-Proof.
-  split.
-  - intros peirce X Y H x. apply (peirce _ False). intro nY. exfalso. 
-    apply H; trivial.
-  - apply CP_Peirce.
-Qed.
-
-
-Goal LEM' <=> Peirce.
-Proof.
-  split.
-  - intros lem X Y H. destruct (lem X) as [x | nX].
-    exact x. apply H. intro x. exfalso. apply nX. exact x.
-  - apply Peirce_LEM.
-Qed.
